Intermediate/Decomposition.v
@@ -11,50 +11,116 @@ Require Import Intermediate.PS.
 
 Import Intermediate.
 
+(* iface1 is part of iface2 *)
+Definition part_of (iface1 iface2: Program.interface) : Prop :=
+  forall C CI,
+    PMap.MapsTo C CI iface1 -> PMap.MapsTo C CI iface2.
+
+(* partializing a closed program gives two partial programs which are linkable *)
+Lemma linkability_of_a_partialized_program:
+  forall prog ctx,
+    part_of ctx (prog_interface prog) ->
+    well_formed_program prog ->
+    closed_program prog ->
+    linkable_programs
+      (partialize_program prog ctx)
+      (partialize_program prog (prog_interface (partialize_program prog ctx))).
+Proof.
+Admitted.
+
+(* partializing a closed well-formed program and linking the resulting partial programs
+   gives back the original program *)
+Lemma linking_a_partialized_program:
+  forall prog ctx,
+    part_of ctx (prog_interface prog) ->
+    well_formed_program prog ->
+    closed_program prog ->
+    prog_eq prog
+            (program_link (partialize_program prog ctx)
+                          (partialize_program prog (prog_interface (partialize_program prog ctx)))
+                          (fst (prog_main prog)) (snd (prog_main prog))).
+Proof.
+Admitted.
+
+Corollary init_genv_after_linking_a_partialized_program:
+  forall prog ctx,
+    part_of ctx (prog_interface prog) ->
+    well_formed_program prog ->
+    closed_program prog ->
+    genv_eq (init_genv prog)
+            (init_genv
+               (program_link (partialize_program prog ctx)
+                             (partialize_program prog (prog_interface (partialize_program prog ctx)))
+                             (fst (prog_main prog)) (snd (prog_main prog)))).
+Proof.
+  intros prog ctx Hpart_of Hwell_formedness Hclosedness.
+  apply init_genv_with_same_program.
+  apply linking_a_partialized_program; auto.
+Qed.
+
+(* tricky filtering step *)
+Lemma double_filtering:
+  forall iface1 iface2,
+    part_of iface2 iface1 ->
+    PMap.Equal
+      (PMapExtra.filter
+         (fun k _ => negb (PMap.mem k (PMapExtra.filter
+                                         (fun k' _ => negb (PMap.mem k' iface2))
+                                         iface1)))
+         iface1) iface2.
+Proof.
+Admitted.
+
+Lemma init_genv_with_extension_of_partialized_program:
+  forall prog ctx,
+    part_of ctx (prog_interface prog) ->
+    genv_eq (init_genv prog)
+            (extend_genv (init_genv (partialize_program prog ctx))
+                         (init_genv (partialize_program prog (prog_interface (partialize_program prog ctx))))).
+Proof.
+Admitted.
+
+(* simulations work with program equality *)
+(* is this a problem? Is program equality creating problems here that we have
+   to mix it with CompCert definitions that doesn't care about it? I think it might *)
+Lemma same_program_forward_simulation:
+  forall p p1 ctx,
+    forward_simulation (CS.sem p) (PS.sem p1 ctx) ->
+  forall p2,
+    prog_eq p1 p2 ->
+    forward_simulation (CS.sem p) (PS.sem p2 ctx).
+Proof.
+Admitted.
+
+(* partializing after the linking phase should give back the original partial program *)
+Lemma partialize_after_linking:
+  forall p c,
+    linkable_programs p c ->
+    prog_eq (partialize_program (program_link p c (fst (prog_main p)) (snd (prog_main p)))
+                                (prog_interface c)) p.
+Proof.
+Admitted.
+
 Section Decomposition.
   Variable prog: program.
   Variable ctx: Program.interface.
 
-  (*
+  Hypothesis input_program_well_formedness:
+    well_formed_program prog.
+
   Hypothesis input_program_closedness:
     closed_program prog.
-   *)
 
-  (* might be useful in the future
   Hypothesis context_validity:
-    forall C CI,
-      PMap.MapsTo C CI ctx -> PMap.MapsTo C CI (prog_interface prog).
-   *)
+    part_of ctx (prog_interface prog).
 
-  (* Might be useful in the future:
-  Lemma imported_procedure_in_context:
-    forall C C' P,
-      PMap.In C ctx ->
-      imported_procedure (genv_interface G) C C' P ->
-      imported_procedure ctx C C' P.
-  Proof.
-    intros C C' P Hin_ctx Himport.
-    unfold imported_procedure in *.
-    unfold PMap.In, PMap.Raw.In0 in Hin_ctx.
-    destruct Hin_ctx as [CI HCI].
-    destruct Himport as [CI' [HCI' Himp]].
-    unfold Program.has_component in *.
-    assert (HCI2 := HCI).
-    apply context_validity in HCI.
-    unfold G, init_genv in HCI'.
-    destruct (init_all prog). destruct p. simpl in *.
-    pose proof (PMapFacts.MapsTo_fun HCI HCI'). subst.
-    exists CI'. split; auto.
-  Qed.
-   *)
-
-  Let G: global_env := init_genv prog.
+  Let pprog := partialize_program prog ctx.
 
   Lemma match_initial_states:
     forall ics,
       CS.initial_state prog ics ->
     exists ips,
-      PS.initial_state prog ctx ips /\ PS.partial_state ctx ics ips.
+      PS.initial_state pprog ctx ips /\ PS.partial_state ctx ics ips.
   Proof.
     intros ics Hics_init.
     CS.unfold_states.
@@ -64,24 +130,36 @@ Section Decomposition.
       simpl; rewrite Htarget.
     (* context has control *)
     - split.
-      + econstructor.
+      + eapply PS.initial_state_intro
+          with (p':=partialize_program prog (prog_interface pprog)).
+        * subst pprog.
+          apply linkability_of_a_partialized_program; auto.
         * eapply PS.ContextControl; eauto.
           ** PS.simplify_turn.
              apply PMapFacts.mem_in_iff. auto.
           ** apply PMapFacts.Equal_refl.
-        * eauto.
+        * subst pprog.
+          eapply CS.same_program_initial_state with (p1:=prog).
+          ** simpl. apply linking_a_partialized_program; auto.
+          ** eassumption.
       + eapply PS.ContextControl; eauto.
         ** PS.simplify_turn.
            apply PMapFacts.mem_in_iff. auto.
         ** apply PMapFacts.Equal_refl.
     (* program has control *)
     - split.
-      + econstructor.
+      + eapply PS.initial_state_intro
+          with (p':=partialize_program prog (prog_interface pprog)).
+        * subst pprog.
+          apply linkability_of_a_partialized_program; auto.
         * eapply PS.ProgramControl; auto.
           ** PS.simplify_turn.
              apply PMapFacts.not_mem_in_iff. auto.
           ** apply PMapFacts.Equal_refl.
-        * eauto.
+        * subst pprog.
+          eapply CS.same_program_initial_state with (p1:=prog).
+          ** simpl; apply linking_a_partialized_program; auto.
+          ** eassumption.
       + eapply PS.ProgramControl; auto.
         ** PS.simplify_turn.
            apply PMapFacts.not_mem_in_iff. auto.
@@ -91,8 +169,8 @@ Section Decomposition.
   Lemma match_final_states:
     forall ics ips,
       PS.partial_state ctx ics ips ->
-      CS.final_state G ics ->
-      PS.final_state prog ctx ips.
+      CS.final_state (init_genv prog) ics ->
+      PS.final_state pprog ctx ips.
   Proof.
     intros ics ips Hpartial Hics_final.
     CS.unfold_states.
@@ -107,21 +185,27 @@ Section Decomposition.
         PS.simplify_turn. auto.
     (* program has control *)
     - inversion Hpartial; inversion H; subst.
-      + eapply PS.final_state_program.
+      + eapply PS.final_state_program
+          with (p':=partialize_program prog (prog_interface pprog)).
+        * subst pprog.
+          apply linkability_of_a_partialized_program; auto.
         * PS.simplify_turn. auto.
         * eauto.
-        * eauto.
+        * subst pprog.
+          eapply CS.same_genv_final_state with (G1:=init_genv prog).
+          ** simpl; apply init_genv_after_linking_a_partialized_program; auto.
+          ** assumption.
       + apply PMapFacts.not_mem_in_iff in Htarget.
         contradiction.
   Qed.
 
   Lemma lockstep_simulation:
     forall ics t ics',
-      CS.step G ics t ics' ->
+      CS.step (init_genv prog) ics t ics' ->
     forall ips,
       PS.partial_state ctx ics ips ->
     exists ips',
-      PS.step ctx G ips t ips' /\ PS.partial_state ctx ics' ips'.
+      PS.step ctx (init_genv pprog) ips t ips' /\ PS.partial_state ctx ics' ips'.
   Proof.
     intros ics t ics' Hstep ips Hpartial.
 
@@ -139,8 +223,40 @@ Section Decomposition.
     (* epsilon steps *)
 
     - eexists. split.
+      + eapply PS.partial_step
+          with (p':=partialize_program prog (prog_interface pprog)); auto.
+        * subst pprog. simpl.
+          apply double_filtering; auto.
+        * apply CS.equal_genvs_step with (G1:=init_genv prog).
+          ** subst pprog. apply init_genv_with_extension_of_partialized_program; auto.
+          ** eassumption.
+        * econstructor; eauto.
+        * econstructor; eauto.
+          ** PS.simplify_turn.
+             rewrite Pointer.inc_preserves_component. auto.
+          ** match goal with
+             | Hmem_eq: PMap.Equal ?MEM1 ?MEM0 |-
+               PMap.Equal _ (PMapExtra.filter _ ?MEM1) =>
+               eapply Memory.equivalence_under_filter;
+               symmetry; apply Hmem_eq
+             end.
       + econstructor; auto.
-        * apply Hstep.
+        ** PS.simplify_turn.
+           rewrite Pointer.inc_preserves_component. auto.
+        ** match goal with
+           | Hmem_eq: PMap.Equal ?MEM1 ?MEM0 |-
+             PMap.Equal _ (PMapExtra.filter _ ?MEM1) =>
+             eapply Memory.equivalence_under_filter;
+             symmetry; apply Hmem_eq
+           end.
+
+    - eexists. split.
+      + eapply PS.partial_step
+          with (p':=partialize_program prog (prog_interface pprog)); auto.
+        * apply double_filtering; auto.
+        * apply CS.equal_genvs_step with (G1:=init_genv prog).
+          ** apply init_genv_with_extension_of_partialized_program; auto.
+          ** eassumption.
         * econstructor; auto.
         * econstructor; eauto.
           ** PS.simplify_turn.
@@ -162,8 +278,12 @@ Section Decomposition.
            end.
 
     - eexists. split.
-      + econstructor; auto.
-        * apply Hstep.
+      + eapply PS.partial_step
+          with (p':=partialize_program prog (prog_interface pprog)); auto.
+        * apply double_filtering; auto.
+        * apply CS.equal_genvs_step with (G1:=init_genv prog).
+          ** apply init_genv_with_extension_of_partialized_program; auto.
+          ** eassumption.
         * econstructor; auto.
         * econstructor; eauto.
           ** PS.simplify_turn.
@@ -185,8 +305,12 @@ Section Decomposition.
            end.
 
     - eexists. split.
-      + econstructor; auto.
-        * apply Hstep.
+      + eapply PS.partial_step
+          with (p':=partialize_program prog (prog_interface pprog)); auto.
+        * apply double_filtering; auto.
+        * apply CS.equal_genvs_step with (G1:=init_genv prog).
+          ** apply init_genv_with_extension_of_partialized_program; auto.
+          ** eassumption.
         * econstructor; auto.
         * econstructor; eauto.
           ** PS.simplify_turn.
@@ -208,8 +332,12 @@ Section Decomposition.
            end.
 
     - eexists. split.
-      + econstructor; auto.
-        * apply Hstep.
+      + eapply PS.partial_step
+          with (p':=partialize_program prog (prog_interface pprog)); auto.
+        * apply double_filtering; auto.
+        * apply CS.equal_genvs_step with (G1:=init_genv prog).
+          ** apply init_genv_with_extension_of_partialized_program; auto.
+          ** eassumption.
         * econstructor; auto.
         * econstructor; eauto.
           ** PS.simplify_turn.
@@ -231,31 +359,12 @@ Section Decomposition.
            end.
 
     - eexists. split.
-      + econstructor; auto.
-        * apply Hstep.
-        * econstructor; auto.
-        * econstructor; eauto.
-          ** PS.simplify_turn.
-             rewrite Pointer.inc_preserves_component. auto.
-          ** match goal with
-             | Hmem_eq: PMap.Equal ?MEM1 ?MEM0 |-
-               PMap.Equal _ (PMapExtra.filter _ ?MEM1) =>
-               eapply Memory.equivalence_under_filter;
-               symmetry; apply Hmem_eq
-             end.
-      + econstructor; auto.
-        ** PS.simplify_turn.
-           rewrite Pointer.inc_preserves_component. auto.
-        ** match goal with
-           | Hmem_eq: PMap.Equal ?MEM1 ?MEM0 |-
-             PMap.Equal _ (PMapExtra.filter _ ?MEM1) =>
-             eapply Memory.equivalence_under_filter;
-             symmetry; apply Hmem_eq
-           end.
-
-    - eexists. split.
-      + econstructor; auto.
-        * apply Hstep.
+      + eapply PS.partial_step
+          with (p':=partialize_program prog (prog_interface pprog)); auto.
+        * apply double_filtering; auto.
+        * apply CS.equal_genvs_step with (G1:=init_genv prog).
+          ** apply init_genv_with_extension_of_partialized_program; auto.
+          ** eassumption.
         * econstructor; auto.
         * econstructor; eauto.
           ** PS.simplify_turn.
@@ -281,8 +390,12 @@ Section Decomposition.
         exists (PS.partialize (gps0, mem', regs0, Pointer.inc pc0) ctx).
         simpl. rewrite Pointer.inc_preserves_component, H.
         split.
-        * econstructor; auto.
-          ** apply Hstep.
+        * eapply PS.partial_step
+            with (p':=partialize_program prog (prog_interface pprog)); auto.
+          ** apply double_filtering; auto.
+          ** apply CS.equal_genvs_step with (G1:=init_genv prog).
+             *** apply init_genv_with_extension_of_partialized_program; auto.
+             *** eassumption.
           ** econstructor; eauto.
              *** PS.simplify_turn; apply PMapFacts.not_mem_in_iff; auto.
           ** econstructor; auto.
@@ -305,8 +418,12 @@ Section Decomposition.
         assumption.
 
     - eexists. split.
-      + econstructor; auto.
-        * apply Hstep.
+      + eapply PS.partial_step
+          with (p':=partialize_program prog (prog_interface pprog)); auto.
+        * apply double_filtering; auto.
+        * apply CS.equal_genvs_step with (G1:=init_genv prog).
+          ** apply init_genv_with_extension_of_partialized_program; auto.
+          ** eassumption.
         * econstructor; auto.
         * econstructor; eauto.
           ** PS.simplify_turn.
@@ -328,8 +445,12 @@ Section Decomposition.
            end.
 
     - eexists. split.
-      + econstructor; auto.
-        * apply Hstep.
+      + eapply PS.partial_step
+          with (p':=partialize_program prog (prog_interface pprog)); auto.
+        * apply double_filtering; auto.
+        * apply CS.equal_genvs_step with (G1:=init_genv prog).
+          ** apply init_genv_with_extension_of_partialized_program; auto.
+          ** eassumption.
         * econstructor; auto.
         * econstructor; eauto.
           ** PS.simplify_turn.
@@ -357,8 +478,12 @@ Section Decomposition.
            end.
 
     - eexists. split.
-      + econstructor; auto.
-        * apply Hstep.
+      + eapply PS.partial_step
+          with (p':=partialize_program prog (prog_interface pprog)); auto.
+        * apply double_filtering; auto.
+        * apply CS.equal_genvs_step with (G1:=init_genv prog).
+          ** apply init_genv_with_extension_of_partialized_program; auto.
+          ** eassumption.
         * econstructor; auto.
         * econstructor; eauto.
           ** PS.simplify_turn.
@@ -380,8 +505,12 @@ Section Decomposition.
            end.
 
     - eexists. split.
-      + econstructor; auto.
-        * apply Hstep.
+      + eapply PS.partial_step
+          with (p':=partialize_program prog (prog_interface pprog)); auto.
+        * apply double_filtering; auto.
+        * apply CS.equal_genvs_step with (G1:=init_genv prog).
+          ** apply init_genv_with_extension_of_partialized_program; auto.
+          ** eassumption.
         * econstructor; auto.
         * econstructor; eauto.
           ** PS.simplify_turn.
@@ -408,8 +537,12 @@ Section Decomposition.
         exists (PS.partialize (gps0, mem', Register.set rptr (Ptr ptr) regs0, Pointer.inc pc0) ctx).
         simpl. rewrite Pointer.inc_preserves_component, H.
         split.
-        * econstructor; auto.
-          ** apply Hstep.
+        * eapply PS.partial_step
+            with (p':=partialize_program prog (prog_interface pprog)); auto.
+          ** apply double_filtering; auto.
+          ** apply CS.equal_genvs_step with (G1:=init_genv prog).
+             *** apply init_genv_with_extension_of_partialized_program; auto.
+             *** eassumption.
           ** econstructor; eauto.
              *** PS.simplify_turn; apply PMapFacts.not_mem_in_iff in H; auto.
           ** econstructor; eauto.
@@ -439,8 +572,12 @@ Section Decomposition.
     - destruct (PMap.mem C' ctx) eqn:Htarget.
       (* external call *)
       + eexists. split.
-        * econstructor; auto.
-          ** apply Hstep.
+        * eapply PS.partial_step
+            with (p':=partialize_program prog (prog_interface pprog)); auto.
+          ** apply double_filtering; auto.
+          ** apply CS.equal_genvs_step with (G1:=init_genv prog).
+             *** apply init_genv_with_extension_of_partialized_program; auto.
+             *** eassumption.
           ** eapply PS.ProgramControl; auto.
           ** eapply PS.ContextControl; auto.
              *** PS.simplify_turn.
@@ -462,8 +599,12 @@ Section Decomposition.
              end.
       (* internal call *)
       + eexists. split.
-        * econstructor; auto.
-          ** apply Hstep.
+        * eapply PS.partial_step
+            with (p':=partialize_program prog (prog_interface pprog)); auto.
+          ** apply double_filtering; auto.
+          ** apply CS.equal_genvs_step with (G1:=init_genv prog).
+             *** apply init_genv_with_extension_of_partialized_program; auto.
+             *** eassumption.
           ** eapply PS.ProgramControl; auto.
           ** eapply PS.ProgramControl; auto.
              *** PS.simplify_turn.
@@ -489,8 +630,12 @@ Section Decomposition.
     - destruct (PMap.mem (Pointer.component pc') ctx) eqn:Htarget.
       (* external return *)
       + eexists. split.
-        * econstructor; auto.
-          ** apply Hstep.
+        * eapply PS.partial_step
+            with (p':=partialize_program prog (prog_interface pprog)); auto.
+          ** apply double_filtering; auto.
+          ** apply CS.equal_genvs_step with (G1:=init_genv prog).
+             *** apply init_genv_with_extension_of_partialized_program; auto.
+             *** eassumption.
           ** eapply PS.ProgramControl; auto.
           ** eapply PS.ContextControl; auto.
              *** PS.simplify_turn.
@@ -512,8 +657,12 @@ Section Decomposition.
              end.
       (* internal return *)
       + eexists. split.
-        * econstructor; auto.
-          ** apply Hstep.
+        * eapply PS.partial_step
+            with (p':=partialize_program prog (prog_interface pprog)); auto.
+          ** apply double_filtering; auto.
+          ** apply CS.equal_genvs_step with (G1:=init_genv prog).
+             *** apply init_genv_with_extension_of_partialized_program; auto.
+             *** eassumption.
           ** eapply PS.ProgramControl; auto.
           ** eapply PS.ProgramControl; auto.
              *** PS.simplify_turn.
@@ -539,8 +688,12 @@ Section Decomposition.
     (* epsilon steps *)
 
     - eexists. split.
-      + econstructor; auto.
-        * apply Hstep.
+      + eapply PS.partial_step
+          with (p':=partialize_program prog (prog_interface pprog)); auto.
+        * apply double_filtering; auto.
+        * apply CS.equal_genvs_step with (G1:=init_genv prog).
+          ** apply init_genv_with_extension_of_partialized_program; auto.
+          ** eassumption.
         * eapply PS.ContextControl;
             try reflexivity.
           ** PS.simplify_turn. auto.
@@ -555,8 +708,12 @@ Section Decomposition.
            rewrite Pointer.inc_preserves_component. auto.
 
     - eexists. split.
-      + econstructor; auto.
-        * apply Hstep.
+      + eapply PS.partial_step
+          with (p':=partialize_program prog (prog_interface pprog)); auto.
+        * apply double_filtering; auto.
+        * apply CS.equal_genvs_step with (G1:=init_genv prog).
+          ** apply init_genv_with_extension_of_partialized_program; auto.
+          ** eassumption.
         * eapply PS.ContextControl;
             try reflexivity.
           ** PS.simplify_turn. auto.
@@ -571,8 +728,12 @@ Section Decomposition.
            rewrite Pointer.inc_preserves_component. auto.
 
     - eexists. split.
-      + econstructor; auto.
-        * apply Hstep.
+      + eapply PS.partial_step
+          with (p':=partialize_program prog (prog_interface pprog)); auto.
+        * apply double_filtering; auto.
+        * apply CS.equal_genvs_step with (G1:=init_genv prog).
+          ** apply init_genv_with_extension_of_partialized_program; auto.
+          ** eassumption.
         * eapply PS.ContextControl;
             try reflexivity.
           ** PS.simplify_turn. auto.
@@ -587,8 +748,12 @@ Section Decomposition.
            rewrite Pointer.inc_preserves_component. auto.
 
     - eexists. split.
-      + econstructor; auto.
-        * apply Hstep.
+      + eapply PS.partial_step
+          with (p':=partialize_program prog (prog_interface pprog)); auto.
+        * apply double_filtering; auto.
+        * apply CS.equal_genvs_step with (G1:=init_genv prog).
+          ** apply init_genv_with_extension_of_partialized_program; auto.
+          ** eassumption.
         * eapply PS.ContextControl;
             try reflexivity.
           ** PS.simplify_turn. auto.
@@ -603,8 +768,12 @@ Section Decomposition.
            rewrite Pointer.inc_preserves_component. auto.
 
     - eexists. split.
-      + econstructor; auto.
-        * apply Hstep.
+      + eapply PS.partial_step
+          with (p':=partialize_program prog (prog_interface pprog)); auto.
+        * apply double_filtering; auto.
+        * apply CS.equal_genvs_step with (G1:=init_genv prog).
+          ** apply init_genv_with_extension_of_partialized_program; auto.
+          ** eassumption.
         * eapply PS.ContextControl;
             try reflexivity.
           ** PS.simplify_turn. auto.
@@ -619,8 +788,12 @@ Section Decomposition.
            rewrite Pointer.inc_preserves_component. auto.
 
     - eexists. split.
-      + econstructor; auto.
-        * apply Hstep.
+      + eapply PS.partial_step
+          with (p':=partialize_program prog (prog_interface pprog)); auto.
+        * apply double_filtering; auto.
+        * apply CS.equal_genvs_step with (G1:=init_genv prog).
+          ** apply init_genv_with_extension_of_partialized_program; auto.
+          ** eassumption.
         * eapply PS.ContextControl;
             try reflexivity.
           ** PS.simplify_turn. auto.
@@ -635,8 +808,12 @@ Section Decomposition.
            rewrite Pointer.inc_preserves_component. auto.
 
     - eexists. split.
-      + econstructor; auto.
-        * apply Hstep.
+      + eapply PS.partial_step
+          with (p':=partialize_program prog (prog_interface pprog)); auto.
+        * apply double_filtering; auto.
+        * apply CS.equal_genvs_step with (G1:=init_genv prog).
+          ** apply init_genv_with_extension_of_partialized_program; auto.
+          ** eassumption.
         * eapply PS.ContextControl;
             try reflexivity.
           ** PS.simplify_turn. auto.
@@ -651,8 +828,12 @@ Section Decomposition.
            rewrite Pointer.inc_preserves_component. auto.
 
     - eexists. split.
-      + econstructor; auto.
-        * apply Hstep.
+      + eapply PS.partial_step
+          with (p':=partialize_program prog (prog_interface pprog)); auto.
+        * apply double_filtering; auto.
+        * apply CS.equal_genvs_step with (G1:=init_genv prog).
+          ** apply init_genv_with_extension_of_partialized_program; auto.
+          ** eassumption.
         * eapply PS.ContextControl;
             try reflexivity.
           ** PS.simplify_turn. auto.
@@ -667,8 +848,12 @@ Section Decomposition.
            erewrite <- find_label_in_component_1; eauto.
 
     - eexists. split.
-      + econstructor; auto.
-        * apply Hstep.
+      + eapply PS.partial_step
+          with (p':=partialize_program prog (prog_interface pprog)); auto.
+        * apply double_filtering; auto.
+        * apply CS.equal_genvs_step with (G1:=init_genv prog).
+          ** apply init_genv_with_extension_of_partialized_program; auto.
+          ** eassumption.
         * eapply PS.ContextControl;
             try reflexivity.
           ** PS.simplify_turn. auto.
@@ -683,8 +868,12 @@ Section Decomposition.
            rewrite H4. auto.
 
     - eexists. split.
-      + econstructor; auto.
-        * apply Hstep.
+      + eapply PS.partial_step
+          with (p':=partialize_program prog (prog_interface pprog)); auto.
+        * apply double_filtering; auto.
+        * apply CS.equal_genvs_step with (G1:=init_genv prog).
+          ** apply init_genv_with_extension_of_partialized_program; auto.
+          ** eassumption.
         * eapply PS.ContextControl;
             try reflexivity.
           ** PS.simplify_turn. auto.
@@ -699,8 +888,12 @@ Section Decomposition.
            erewrite <- find_label_in_procedure_1; eauto.
 
     - eexists. split.
-      + econstructor; auto.
-        * apply Hstep.
+      + eapply PS.partial_step
+          with (p':=partialize_program prog (prog_interface pprog)); auto.
+        * apply double_filtering; auto.
+        * apply CS.equal_genvs_step with (G1:=init_genv prog).
+          ** apply init_genv_with_extension_of_partialized_program; auto.
+          ** eassumption.
         * eapply PS.ContextControl;
             try reflexivity.
           ** PS.simplify_turn. auto.
@@ -715,8 +908,12 @@ Section Decomposition.
            rewrite Pointer.inc_preserves_component. auto.
 
     - eexists. split.
-      + econstructor; auto.
-        * apply Hstep.
+      + eapply PS.partial_step
+          with (p':=partialize_program prog (prog_interface pprog)); auto.
+        * apply double_filtering; auto.
+        * apply CS.equal_genvs_step with (G1:=init_genv prog).
+          ** apply init_genv_with_extension_of_partialized_program; auto.
+          ** eassumption.
         * eapply PS.ContextControl;
             try reflexivity.
           ** PS.simplify_turn. auto.
@@ -735,8 +932,12 @@ Section Decomposition.
     - destruct (PMap.mem C' ctx) eqn:Htarget.
       (* internal call *)
       + eexists. split.
-        * econstructor; auto.
-          ** apply Hstep.
+        * eapply PS.partial_step
+            with (p':=partialize_program prog (prog_interface pprog)); auto.
+          ** apply double_filtering; auto.
+          ** apply CS.equal_genvs_step with (G1:=init_genv prog).
+             *** apply init_genv_with_extension_of_partialized_program; auto.
+             *** eassumption.
           ** eapply PS.ContextControl; auto.
           ** eapply PS.ContextControl; auto.
              *** PS.simplify_turn.
@@ -758,8 +959,12 @@ Section Decomposition.
              end.
       (* external call *)
       + eexists. split.
-        * econstructor; auto.
-          ** apply Hstep.
+        * eapply PS.partial_step
+            with (p':=partialize_program prog (prog_interface pprog)); auto.
+          ** apply double_filtering; auto.
+          ** apply CS.equal_genvs_step with (G1:=init_genv prog).
+             *** apply init_genv_with_extension_of_partialized_program; auto.
+             *** eassumption.
           ** eapply PS.ContextControl; auto.
           ** eapply PS.ProgramControl; auto.
              *** PS.simplify_turn.
@@ -785,8 +990,12 @@ Section Decomposition.
     - destruct (PMap.mem (Pointer.component pc') ctx) eqn:Htarget.
       (* internal return *)
       + eexists. split.
-        * econstructor; auto.
-          ** apply Hstep.
+        * eapply PS.partial_step
+            with (p':=partialize_program prog (prog_interface pprog)); auto.
+          ** apply double_filtering; auto.
+          ** apply CS.equal_genvs_step with (G1:=init_genv prog).
+             *** apply init_genv_with_extension_of_partialized_program; auto.
+             *** eassumption.
           ** eapply PS.ContextControl; auto.
           ** eapply PS.ContextControl; auto.
              *** PS.simplify_turn.
@@ -808,8 +1017,12 @@ Section Decomposition.
              end.
       (* external return *)
       + eexists. split.
-        * econstructor; auto.
-          ** apply Hstep.
+        * eapply PS.partial_step
+            with (p':=partialize_program prog (prog_interface pprog)); auto.
+          ** apply double_filtering; auto.
+          ** apply CS.equal_genvs_step with (G1:=init_genv prog).
+             *** apply init_genv_with_extension_of_partialized_program; auto.
+             *** eassumption.
           ** eapply PS.ContextControl; auto.
           ** eapply PS.ProgramControl; auto.
              *** PS.simplify_turn.
@@ -832,7 +1045,7 @@ Section Decomposition.
   Qed.
 
   Theorem decomposition:
-    forward_simulation (CS.sem prog) (PS.sem prog ctx).
+    forward_simulation (CS.sem prog) (PS.sem pprog ctx).
   Proof.
     eapply forward_simulation_step.
     - apply match_initial_states.
@@ -842,7 +1055,7 @@ Section Decomposition.
 
   Corollary decomposition_with_refinement:
     forall beh1, program_behaves (CS.sem prog) beh1 ->
-    exists beh2, program_behaves (PS.sem prog ctx) beh2 /\ behavior_improves beh1 beh2.
+    exists beh2, program_behaves (PS.sem pprog ctx) beh2 /\ behavior_improves beh1 beh2.
   Proof.
     intros beh1 Hbeh1.
     eapply forward_simulation_behavior_improves; eauto.
@@ -852,14 +1065,34 @@ End Decomposition.
 
 Section DecompositionAndLinking.
   Variable p c: program.
-  Variable mainC: Component.id.
-  Variable mainP: Procedure.id.
 
-  Corollary decomposition_with_linking:    
-    forward_simulation (CS.sem (program_link p c mainC mainP))
-                       (PS.sem (program_link p c mainC mainP)
-                               (prog_interface c)).
+  Hypothesis linkability:
+    linkable_programs p c.
+
+  Hypothesis closedness_after_linking:
+    closed_program (program_link p c (fst (prog_main p)) (snd (prog_main p))).
+
+  Lemma context_validity:
+    part_of (prog_interface c)
+            (prog_interface (program_link p c (fst (prog_main p)) (snd (prog_main p)))).
   Proof.
-    apply decomposition.
+    unfold part_of.
+    intros C CI Hin.
+    simpl.
+    apply PMapExtra.update_mapsto_iff. left.
+    assumption.
+  Qed.
+
+  Corollary decomposition_with_linking:
+    forward_simulation (CS.sem (program_link p c (fst (prog_main p)) (snd (prog_main p))))
+                       (PS.sem p (prog_interface c)).
+  Proof.
+    eapply same_program_forward_simulation.
+    - eapply decomposition.
+      + apply (linking_well_formedness p c (fst (prog_main p)) (snd (prog_main p))
+                                       linkability).
+      + assumption.
+      + apply context_validity.
+    - apply partialize_after_linking; auto.
   Qed.
 End DecompositionAndLinking.
