Intermediate/GlobalEnv.v
@@ -11,6 +11,52 @@ Record global_env := mkGlobalEnv {
   genv_entrypoints: EntryPoint.t;
 }.
 
+Inductive genv_eq : global_env -> global_env -> Prop :=
+| genv_eq_intro: forall iface1 procs1 eps1 iface2 procs2 eps2,
+    PMap.Equal iface1 iface2 ->
+    PMap.Equal procs1 procs2 ->
+    PMap.Equal eps1 eps2 ->
+    genv_eq (mkGlobalEnv iface1 procs1 eps1) (mkGlobalEnv iface2 procs2 eps2).
+
+Lemma genv_eq_refl:
+  forall G,
+    genv_eq G G.
+Proof.
+  intros G.
+  destruct G.
+  constructor; reflexivity.
+Qed.
+
+Lemma genv_eq_sym:
+  forall G1 G2,
+    genv_eq G1 G2 -> genv_eq G2 G1.
+Proof.
+  intros G1 G2 H.
+  destruct G1. destruct G2.
+  inversion H; subst.
+  constructor;
+    try reflexivity;
+    try symmetry; assumption.
+Qed.
+
+Lemma genv_eq_trans:
+  forall G1 G2 G3,
+    genv_eq G1 G2 -> genv_eq G2 G3 -> genv_eq G1 G3.
+Proof.
+  intros G1 G2 G3 H1 H2.
+  destruct G1. destruct G2. destruct G3.
+  inversion H1; subst; inversion H2; subst;
+    constructor;
+    try reflexivity;
+    try etransitivity; eauto.
+Qed.
+
+Add Parametric Relation: (global_env) (genv_eq)
+    reflexivity proved by (genv_eq_refl)
+    symmetry proved by (genv_eq_sym)
+    transitivity proved by (genv_eq_trans)
+      as genv_eq_rel.
+
 Record well_formed_global_env (G: global_env) := {
   (* the interface is sound (but maybe not closed) *)
   wfgenv_interface_soundness:
@@ -29,12 +75,39 @@ Definition init_genv (p: program) : global_env :=
      genv_procedures := ps;
      genv_entrypoints := E |}.
 
+Definition extend_genv (G1: global_env) (G2: global_env) : global_env :=
+  {| genv_interface := PMapExtra.update (genv_interface G1) (genv_interface G2);
+     genv_procedures := PMapExtra.update (genv_procedures G1) (genv_procedures G2);
+     genv_entrypoints := PMapExtra.update (genv_entrypoints G1) (genv_entrypoints G2) |}.
+
 Definition executing G (pc : Pointer.t) (i : instr) : Prop :=
   exists C_procs P_code,
     PMap.find (Pointer.component pc) (genv_procedures G) = Some C_procs /\
     PMap.find (Pointer.block pc) C_procs = Some P_code /\
     Pointer.offset pc >= 0 /\
     nth_error P_code (Z.to_nat (Pointer.offset pc)) = Some i.
+
+Lemma execution_in_same_environment:
+  forall G1 G2 pc i,
+    genv_eq G1 G2 ->
+    executing G1 pc i ->
+    executing G2 pc i.
+Proof.
+Admitted.
+
+Lemma init_genv_with_same_program:
+  forall p1 p2,
+    prog_eq p1 p2 ->
+    genv_eq (init_genv p1) (init_genv p2).
+Proof.
+  intros p1 p2 Heq.
+  unfold init_genv.
+  pose proof (init_all_with_same_program p1 p2).
+  destruct (init_all p1) as [[]].
+  destruct (init_all p2) as [[]].
+  destruct (H Heq) as [? []].
+  constructor.
+Admitted.
 
 Fixpoint find_label (c : code) (l : label) : option Z :=
   let fix aux c o :=
